core(sort): Generalize basic support for orderby
Signed-off-by: Jerome Simeon <jeromesimeon@me.com>

compiler/core/Data/Operators/SortBy.v
@@ -25,72 +25,42 @@ Require Import ForeignData.
 Require Import Data.
 Require Import DataNorm.
 
+(* For data *)
 Section SortBy.
   Context {fdata:foreign_data}.
-  
-  (* Eval vm_compute in (sort_sortable_coll scoll1). *)
-  
-  Definition get_criteria (d:data) (sc:SortCriteria) : option sdata :=
-    let (att,sk) := sc in (* XXX IGNORES sort kind (asc|desc) XXX *)
+
+  Definition sdata_of_data (d:data) : option sdata :=
     match d with
-    | drec r =>
-      match edot r att with
-      | Some (dnat n) => Some (sdnat n)
-      | Some (dstring s) => Some (sdstring s)
-      | Some _ => None
-      | None => None
-      end
+    | dnat n => Some (sdnat n)
+    | dstring s => Some (sdstring s)
     | _ => None
     end.
-
-  Definition get_criterias (d:data) (scl:SortCriterias) : option (list sdata) :=
-    lift_map (get_criteria d) scl.
-
-  Definition sortable_data_of_data (d:data) (scl:SortCriterias) : option sortable_data :=
-    lift (fun c => (c,d)) (get_criterias d scl).
-
-  Definition sortable_coll_of_coll (scl:SortCriterias) (coll:list data) :
-    option (list sortable_data)
-    := lift_map (fun d => sortable_data_of_data d scl) coll.
   
-  Definition data_sort (scl:SortCriterias) (d:data) : option data :=
+  Definition get_criteria (sc:SortCriteria) (r:list (string * data)) : option sdata :=
+    let (att,sk) := sc in (* XXX IGNORES sort kind (asc|desc) XXX *)
+    match edot r att with
+    | Some d => sdata_of_data d
+    | None => None
+    end.
+
+  Definition table_of_data (d:data) : option (list (list (string * data))):=
     match d with
     | dcoll coll =>
-      lift dcoll
-           (lift coll_of_sortable_coll
-                 (lift sort_sortable_coll
-                       (sortable_coll_of_coll scl coll)))
+      lift_map (fun d =>
+                  match d with
+                  | drec r => Some r
+                  | _ => None
+                  end) coll
     | _ => None
     end.
 
-  (* Example *)
-  Definition mkperson (name:string) (age:Z) (zip:Z) (company:string) :=
-    drec (("name", dstring name)
-          :: ("age", dnat age)
-          :: ("zip", dnat zip)
-          :: ("company", dstring company)
-          :: nil)%string.
-  Definition mkpersons_aux l :=
-    map (fun x =>
-           match x with (name, age, zip, company) => mkperson name age zip company
-           end) l.
-  Definition mkpersons l :=
-    dcoll (mkpersons_aux l).
-
-  Open Scope Z_scope.
-  Definition persons :=
-    mkpersons
-      (("John",23,1008,"ACME")
-         :: ("Jane",24,1009,"AIGO")
-         :: ("Jill",25,1010,"ACME")
-         :: ("Jack",27,1010,"CMUD")
-         :: nil)%string.
-
-  (*
-  Eval vm_compute in persons.
-  Eval vm_compute in (data_sort (("name"%string,Ascending)::nil) persons).
-  Eval vm_compute in (data_sort (("zip"%string,Ascending)::("name"%string,Ascending)::nil) persons).
-  *)
+  Definition data_of_table (t: list (list (string * data))) : data :=
+    dcoll (map drec t).
+  
+  Definition data_sort
+             (scl:list (list (string * data) -> option sdata))
+             (d:data) : option data :=
+    lift data_of_table (olift (table_sort scl) (table_of_data d)).
 
 End SortBy.
 
@@ -99,13 +69,27 @@ Section SortByProps.
 
   Lemma sortable_data_normalized h a sc sd :
     data_normalized h a ->
-    sortable_data_of_data a sc = Some sd ->
+    fsortable_data_of_data a sc = Some sd ->
     data_normalized h (snd sd).
   Proof.
-    unfold sortable_data_of_data; intros dn eqs.
+    unfold fsortable_data_of_data; intros dn eqs.
     apply some_lift in eqs.
     destruct eqs as [? eqs ?]; subst.
     simpl; trivial.
+  Qed.
+
+  Lemma fsortable_data_of_data_snd_inv {A:Set} (l0: list (string * A))
+        (s:list (list (string * A) -> option sdata)) (s0:sortable_data) :
+    fsortable_data_of_data l0 s = Some s0 ->
+    l0 = snd s0.
+  Proof.
+    intros.
+    destruct s0; simpl in *.
+    unfold fsortable_data_of_data in H.
+    unfold lift in H.
+    destruct (fget_criterias l0 s); try discriminate.
+    inversion H.
+    reflexivity.
   Qed.
 
   Lemma data_sort_normalized h s (d sd:data) :
@@ -118,30 +102,65 @@ Section SortByProps.
     intros dn; invcs dn.
     constructor.
     rewrite Forall_forall in *.
+    simpl in eqs.
+    unfold table_sort in eqs.
     revert x eqs H0.
     induction l; simpl; intros x eqs dn d ind.
-    - unfold sortable_coll_of_coll in eqs.
-      simpl in eqs.
-      invcs eqs.
+    - invcs eqs.
       simpl in *; tauto.
-    - unfold sortable_coll_of_coll in *.
-      simpl in eqs.
-      case_eq (sortable_data_of_data a s)
-      ; [intros ? eqq1 | intros eqq1]; rewrite eqq1 in eqs
-      ; try discriminate.
-      case_eq (lift_map (fun d : data => sortable_data_of_data d s) l)
+    - destruct a; simpl in *; try discriminate.
+      case_eq (lift_map (fun d : data => match d with
+                                        | drec r => Some r
+                                        | _ => None
+                                        end) l);
+        [intros ? eqq1 | intros eqq1]; rewrite eqq1 in eqs
+        ; rewrite eqq1 in IHl
+        ; try discriminate; simpl in *.
+      unfold fsortable_coll_of_coll in *; simpl in eqs.
+      unfold lift in eqs.
+      case_eq (fsortable_data_of_data l0 s)
       ; [intros ? eqq2 | intros eqq2]; rewrite eqq2 in eqs
       ; try discriminate.
-      invcs eqs.
-      assert (dnimpl:(forall x : data, In x l -> data_normalized h x)) by auto.
-      specialize (IHl _ eqq2 dnimpl).
-      rewrite in_csc_ssc in ind.
-      destruct ind.
+      case_eq (lift_map (fun d : list (string * data) => fsortable_data_of_data d s) l1)
+      ; [intros ? eqq3 | intros eqq3]; rewrite eqq3 in eqs
+      ; rewrite eqq3 in IHl
+      ; try discriminate.
+      assert (x = coll_of_sortable_coll (sort_sortable_coll (s0 :: l2)))
+        by (inversion eqs; reflexivity).
+      rewrite H in *; clear H.
+      unfold coll_of_sortable_coll in ind.
+      rewrite map_map in ind.
+      rewrite in_map_iff in ind.
+      elim ind; intros; clear ind.
+      elim H; intros; clear H.
+      rewrite <- H0 in *; clear H0.
+      unfold sort_sortable_coll, dict_sort in H1.
+      inversion eqs; clear eqs.
+      assert (In x0 (s0 :: l2)) by apply (in_insertion_sort _ H1); clear H1;
+        simpl in H.
+      elim H; intros; simpl in *; clear H.
       + subst.
-        eapply sortable_data_normalized; eauto.
-      + rewrite <- in_csc_ssc in H.
-        auto.
+        apply dn.
+        left.
+        unfold fsortable_data_of_data in eqq2.
+        unfold fget_criterias in eqq2.
+        unfold lift in eqq2.
+        case_eq (lift_map (fun f : list (string * data) -> option sdata => f l0) s);
+          intros; rewrite H in *; simpl; try congruence.
+        inversion eqq2; reflexivity.
+      + eapply IHl.
+        reflexivity.
+        * intros.
+          apply (dn x1).
+          right; assumption.
+        * rewrite in_map_iff.
+          exists (snd x0).
+          split; [reflexivity|].
+          rewrite in_csc_ssc.
+          unfold coll_of_sortable_coll.
+          rewrite in_map_iff.
+          exists x0.
+          split; [reflexivity|assumption].
   Qed.
 
 End SortByProps.
-
