compiler/core/EJson/Operators/EJsonSortBy.v
@@ -28,71 +28,32 @@ Section EJsonSortBy.
   Context {foreign_ejson_model:Set}.
   Context {fejson:foreign_ejson foreign_ejson_model}.
 
-  Definition ejson_get_criteria (j:@ejson foreign_ejson_model) (sc:@ejson foreign_ejson_model) : option sdata :=
+  Definition ejson_get_criteria (sc:@ejson foreign_ejson_model) (r:list (string * @ejson foreign_ejson_model)) : option sdata :=
     match sc with
     | ejobject (("asc"%string, ejstring att)::nil)
     | ejobject (("desc"%string, ejstring att)::nil) => (* XXX IGNORES sort kind (asc|desc) XXX *)
-      match ejson_is_record j with
-      | Some r =>
-        match edot r att with
-        | Some (ejbigint n) => Some (sdnat n)
-        | Some (ejstring s) => Some (sdstring s)
-        | Some _ => None
-        | None => None
-        end
+      match edot r att with
+      | Some (ejbigint n) => Some (sdnat n)
+      | Some (ejstring s) => Some (sdstring s)
+      | Some _ => None
       | None => None
       end
     | _ => None
     end.
 
-  Definition ejson_get_criterias (j:ejson) (scl:list ejson) : option (list sdata) :=
-    lift_map (ejson_get_criteria j) scl.
-
-  Definition ejson_sortable_data_of_ejson (j:ejson) (scl:list ejson) : option sortable_data :=
-    lift (fun c => (c,j)) (ejson_get_criterias j scl).
-
-  Definition ejson_sortable_coll_of_coll (scl:list ejson) (coll:list ejson) :
-    option (list sortable_data)
-    := lift_map (fun j => ejson_sortable_data_of_ejson j scl) coll.
-  
-  Definition ejson_sort (scl:list ejson) (j:ejson) : option ejson :=
-    match j with
-    | ejarray coll =>
-      lift ejarray
-           (lift coll_of_sortable_coll
-                 (lift sort_sortable_coll
-                       (ejson_sortable_coll_of_coll scl coll)))
+  Definition table_of_ejson (d:@ejson foreign_ejson_model) : option (list (list (string * ejson))):=
+    match d with
+    | ejarray coll => lift_map ejson_is_record coll
     | _ => None
     end.
 
-  (* Example *)
-  Definition mkperson (name:string) (age:Z) (zip:Z) (company:string) : @ejson foreign_ejson_model :=
-    ejobject (("name", ejstring name)
-                :: ("age", ejbigint age)
-                :: ("zip", ejbigint zip)
-                :: ("company", ejstring company)
-                :: nil)%string.
-  Definition mkpersons_aux l :=
-    map (fun x =>
-           match x with (name, age, zip, company) => mkperson name age zip company
-           end) l.
-  Definition mkpersons l :=
-    ejarray (mkpersons_aux l).
-
-  Open Scope Z_scope.
-  Definition persons :=
-    mkpersons
-      (("John",23,1008,"ACME")
-         :: ("Jane",24,1009,"AIGO")
-         :: ("Jill",25,1010,"ACME")
-         :: ("Jack",27,1010,"CMUD")
-         :: nil)%string.
-
-  (*
-  Eval vm_compute in persons.
-  Eval vm_compute in (ejson_sort ((ejobject (("asc"%string,ejstring "name"%string)::nil)::nil)) persons).
-  Eval vm_compute in (ejson_sort ((ejobject (("asc"%string,ejstring "zip"%string)::nil))::(ejobject (("asc"%string, ejstring "name"%string)::nil))::nil) persons).
-  *)
+  Definition ejson_of_table (t: list (list (string * @ejson foreign_ejson_model))) : ejson :=
+    ejarray (map ejobject t).
+  
+  Definition ejson_sort
+             (scl:list (list (string * @ejson foreign_ejson_model) -> option sdata))
+             (j:ejson) : option ejson :=
+    lift ejson_of_table (olift (table_sort scl) (table_of_ejson j)).
 
 End EJsonSortBy.
 
